iris/SpecUservec.v
@@ -383,7 +383,7 @@ Definition uservec_post `{!riscvGS Σ, !xv6G Σ, !bioslotG Σ, !fileG Σ} `{GEN 
     ut_fork_out f sc_v (tf_of g (ret_pc sepc_v))
       (pv_tf (us_V U') !!! tf_arg_idx 0) cs cs' -∗
     (* ...AND WAIT'S, forwarded the same way -- [SpecUsertrap.ut_wait_out] *)
-    ut_wait_out sc_v (tf_of g (ret_pc sepc_v))
+    ut_wait_out sc_v (tf_of g (ret_pc sepc_v)) M (us_M U')
       (pv_tf (us_V U') !!! tf_arg_idx 0) cs cs' gn pid -∗
     (* ...AND WHAT A RESUME PROVES, forwarded the same way (lane TRAP-ROWS,
        T2(iii) / T4) -- [SpecUsertrap.ut_live_out] *)
